Progress pan_globals proof

pancake/proofs/pan_globalsProofScript.sml
@@ -12,34 +12,39 @@ val _ = set_grammar_ancestry  ["panSem", "pan_globals", "panProps", "panLang"];
 val s = ``s:('a,'ffi) panSem$state``
 
 Definition state_rel_def:
-  state_rel ctxt s t ⇔
+  state_rel ls ctxt s t ⇔
   s.top_addr = t.top_addr - ctxt.globals_size ∧
-  s.locals = t.locals ∧
+  (ls ⇒ s.locals = t.locals) ∧
   s.base_addr = t.base_addr ∧
   s.be = t.be ∧
+  s.eshapes = t.eshapes ∧
+  s.clock = t.clock ∧
   (∀v val.
      FLOOKUP s.globals v = SOME val ⇒
      ∃addr. FLOOKUP ctxt.globals v = SOME(shape_of val, addr) ∧
             mem_load (shape_of val) (t.top_addr - addr) t.memaddrs t.memory = SOME val
   ) ∧
   s.memaddrs ⊆ t.memaddrs ∧
+  s.sh_memaddrs = t.sh_memaddrs ∧
   (∀addr. addr ∈ s.memaddrs ⇒ s.memory addr = t.memory addr) ∧
-  s.ffi = t.ffi
+  s.ffi = t.ffi ∧
+  (∀fname vshapes prog. FLOOKUP s.code fname = SOME (vshapes,prog) ⇒
+           FLOOKUP t.code fname = SOME (vshapes, compile ctxt prog))
 End
 
 Theorem state_rel_mem_load:
-  state_rel ctxt ^s t ∧
+  state_rel ls ctxt ^s t ∧
   mem_load shape w s.memaddrs s.memory = SOME v ⇒
   mem_load shape w t.memaddrs t.memory = SOME v
 Proof
-  ‘(∀shape w sa sm ctxt ^s t v.
-      state_rel ctxt s t ∧
+  ‘(∀shape w sa sm ls ctxt ^s t v.
+      state_rel ls ctxt s t ∧
       sa = s.memaddrs ∧
       sm = s.memory ∧
       mem_load shape w sa sm = SOME v ⇒
       mem_load shape w t.memaddrs t.memory = SOME v) ∧
-   (∀shapes w sa sm ctxt ^s t v.
-      state_rel ctxt s t ∧
+   (∀shapes w sa sm ls ctxt ^s t v.
+      state_rel ls ctxt s t ∧
       sa = s.memaddrs ∧
       sm = s.memory ∧
       mem_loads shapes w sa sm = SOME v ⇒
@@ -58,7 +63,7 @@ QED
 
 Theorem compile_exp_correct:
   ∀s e v ctxt t.
-  state_rel ctxt s t ∧
+  state_rel T ctxt s t ∧
   eval s e = SOME v
   ⇒
   eval t (compile_exp ctxt e) = SOME v
@@ -107,6 +112,313 @@ Proof
       drule_all pan_commonPropsTheory.opt_mmap_mem_func >>
       strip_tac >> gvs[]) >>
   gvs[wordLangTheory.word_op_def,state_rel_def,eval_def,compile_exp_def,AllCaseEqs()]
+QED
+
+Definition good_res_def:
+  good_res(SOME TimeOut) = F ∧
+  good_res(SOME(Return v)) = F ∧
+  good_res(SOME(Exception l v)) = F ∧
+  good_res(SOME(FinalFFI ev)) = F ∧
+  good_res _ = T
+End
+
+val gen_goal =
+  “λcomp (p,s). ∀res ctxt t s'.
+  state_rel T ctxt s t ∧
+  evaluate(p,s) = (res,s') ∧
+  res ≠ SOME Error
+  ⇒
+  ∃t'.
+    evaluate(comp ctxt p,t) = (res,t') ∧
+    state_rel (good_res res) ctxt s' t'”
+
+local
+  val goal = beta_conv ``^gen_goal pan_globals$compile``
+  val ind_thm = panSemTheory.evaluate_ind
+    |> ISPEC goal
+    |> CONV_RULE (DEPTH_CONV PairRules.PBETA_CONV) |> REWRITE_RULE [];
+  fun list_dest_conj tm = if not (is_conj tm) then [tm] else let
+    val (c1,c2) = dest_conj tm in list_dest_conj c1 @ list_dest_conj c2 end
+  val ind_goals = ind_thm |> concl |> dest_imp |> fst |> list_dest_conj
+in
+  fun get_goal s = first (can (find_term (can (match_term (Term [QUOTE s]))))) ind_goals
+  fun compile_tm () = ind_thm |> concl |> rand
+  fun the_ind_thm () = ind_thm
+  val fgoal = beta_conv ``^gen_goal pan_globals$compile``
+end
+
+Theorem compile_Skip_Break_Continue_Annot_Tick:
+  ^(get_goal "compile _ Skip") /\
+  ^(get_goal "compile _ Break") /\
+  ^(get_goal "compile _ Continue") /\
+  ^(get_goal "compile _ (Annot _ _)") /\
+  ^(get_goal "compile _ Tick")
+Proof
+  rpt strip_tac >>
+  gvs[evaluate_def,compile_def,AllCaseEqs(),dec_clock_def,
+      state_rel_def,empty_locals_def]
+QED
+
+Theorem compile_Assign_Local:
+  ^(get_goal "compile _ (Assign Local _ _)")
+Proof
+  rpt strip_tac >>
+  gvs[evaluate_def,compile_def,AllCaseEqs()] >>
+  drule_all_then strip_assume_tac compile_exp_correct >>
+  simp[] >>
+  gvs[state_rel_def]
+QED
+
+Theorem compile_Assign_Global:
+  ^(get_goal "compile _ (Assign Global _ _)")
+Proof
+  cheat
+QED
+
+Theorem state_rel_res_var[local]:
+  state_rel l ctxt s t ∧ state_rel T ctxt s' t' ⇒
+  state_rel l ctxt
+            (s with locals := res_var s.locals (v,FLOOKUP s'.locals v'))
+            (t with locals := res_var t.locals (v,FLOOKUP t'.locals v'))
+Proof
+  rw[state_rel_def]
+QED
+
+Theorem compile_Dec:
+  ^(get_goal "compile _ (Dec _ _ _)")
+Proof
+  rpt strip_tac >>
+  gvs[evaluate_def,compile_def,AllCaseEqs(),UNCURRY_eq_pair] >>
+  drule_all_then strip_assume_tac compile_exp_correct >>
+  simp[PULL_EXISTS] >>
+  irule_at Any state_rel_res_var >>
+  simp[] >>
+  simp[Once CONJ_SYM] >>
+  first_x_assum irule >>
+  gvs[state_rel_def]
+QED
+
+Theorem compile_Store:
+  ^(get_goal "compile _ (Store _ _)")
+Proof
+  cheat
+QED
+
+Theorem compile_StoreByte:
+  ^(get_goal "compile _ (StoreByte _ _)")
+Proof
+  cheat
+QED
+
+Triviality v_neq_v':
+  v ≠ v ^ «'»
+Proof
+  Cases_on ‘v’ >>
+  rw[mlstringTheory.strcat_def,mlstringTheory.concat_def]
+QED
+
+Theorem compile_ShMemLoad_Local:
+  ^(get_goal "compile _ (ShMemLoad _ _ _ _)")
+Proof
+  strip_tac >> Cases
+  >~ [‘Local’]
+  >- (rw[evaluate_def,AllCaseEqs(),compile_def,PULL_EXISTS,lookup_kvar_def] >>
+      drule_all_then strip_assume_tac compile_exp_correct >>
+      gvs[state_rel_def,sh_mem_load_def,AllCaseEqs(),PULL_EXISTS,set_kvar_def,
+          SUBSET_DEF,set_var_def,empty_locals_def])
+  >~ [‘Global’]
+  >- (rw[evaluate_def,AllCaseEqs(),compile_def,PULL_EXISTS,lookup_kvar_def] >>
+      drule_all_then strip_assume_tac compile_exp_correct >>
+      rename1 ‘FLOOKUP _ _ = SOME(Val vv)’ >>
+      ‘∃addr. FLOOKUP ctxt.globals v = SOME(shape_of(Val vv), addr) ∧
+              mem_load (shape_of(Val vv)) (t.top_addr - addr) t.memaddrs t.memory = SOME(Val vv)’
+        by gvs[state_rel_def] >>
+      ‘s.locals = t.locals’ by gvs[state_rel_def] >>
+      ‘s.sh_memaddrs = t.sh_memaddrs’ by gvs[state_rel_def] >>
+      ‘s.ffi = t.ffi’ by gvs[state_rel_def] >>
+      gvs[] >>
+      simp[oneline shape_of_def] >>
+      PURE_CASE_TAC >>
+      gvs[] >>
+      gvs[evaluate_def,eval_def,FLOOKUP_UPDATE,v_neq_v',
+          lookup_kvar_def,sh_mem_load_def,AllCaseEqs(),
+          wordLangTheory.word_op_def,set_kvar_def,set_var_def,set_global_def,
+          mem_stores_def,mem_store_def,mem_load_def,flatten_def]
+      >- cheat
+      >- (gvs[state_rel_def,empty_locals_def,good_res_def] >>
+          rw[fmap_eq_flookup,FLOOKUP_pan_res_var_thm,FLOOKUP_UPDATE])
+      >- cheat
+      >- (gvs[state_rel_def,empty_locals_def,good_res_def] >>
+          rw[fmap_eq_flookup,FLOOKUP_pan_res_var_thm,FLOOKUP_UPDATE]))
+QED
+
+Theorem compile_ShMemStore:
+  ^(get_goal "compile _ (ShMemStore _ _ _)")
+Proof
+  Cases >> rw[] >>
+  gvs[AllCaseEqs(),panSemTheory.evaluate_def,compile_def,
+      oneline nb_op_def,
+      panSemTheory.nb_op_def,panSemTheory.sh_mem_load_def,
+      panSemTheory.sh_mem_store_def,panLangTheory.size_of_shape_def,
+      asmTheory.is_load_def,panLangTheory.store_op_def,
+      localised_prog_def,SF DNF_ss, good_res_def
+      ] >>
+  imp_res_tac compile_exp_correct >>
+  gvs[state_rel_def]
+QED
+
+Theorem compile_Return:
+  ^(get_goal "compile _ (Return _)")
+Proof
+  rw[evaluate_def,compile_def,AllCaseEqs()] >>
+  imp_res_tac compile_exp_correct >>
+  gvs[state_rel_def,empty_locals_def]
+QED
+
+Theorem compile_Raise:
+  ^(get_goal "compile _ (Raise _ _)")
+Proof
+  rw[evaluate_def,compile_def,AllCaseEqs()] >>
+  imp_res_tac compile_exp_correct >>
+  gvs[state_rel_def,empty_locals_def]
+QED
+
+Theorem compile_Seq:
+  ^(get_goal "compile _ (Seq _ _)")
+Proof
+  rw[evaluate_def,compile_def] >>
+  gvs[UNCURRY_eq_pair,AllCaseEqs()] >>
+  first_x_assum drule >>
+  strip_tac >>
+  gvs[good_res_def]
+QED
+
+Theorem compile_If:
+  ^(get_goal "compile _ (If _ _ _)")
+Proof
+  rw[evaluate_def,compile_def] >>
+  gvs[UNCURRY_eq_pair,AllCaseEqs()] >>
+  imp_res_tac compile_exp_correct >>
+  first_x_assum drule >>
+  strip_tac >>
+  gvs[good_res_def] >>
+  rw[] >>
+  fs[]
+QED
+
+Theorem state_rel_dec_clock[local]:
+  state_rel ls ctxt s t ⇒ state_rel ls ctxt (dec_clock s) (dec_clock t)
+Proof
+  rw[state_rel_def,dec_clock_def]
+QED
+
+Theorem compile_While:
+  ^(get_goal "compile _ (While _ _)")
+Proof
+  rpt strip_tac >>
+  qpat_x_assum ‘evaluate (While e c,s) = (res,s1)’ mp_tac >>
+  rw [Once evaluate_def] >>
+  gvs[AllCaseEqs(),compile_def] >>
+  imp_res_tac compile_exp_correct >>
+  simp[] >>
+  gvs[good_res_def]
+  >- gvs[state_rel_def,empty_locals_def, Once evaluate_def]
+  >- gvs[state_rel_def,empty_locals_def, Once evaluate_def] >>
+  ‘s.clock = t.clock’ by gvs[state_rel_def] >>
+  PURE_ONCE_REWRITE_TAC[evaluate_def] >>
+  simp[] >>
+  imp_res_tac state_rel_dec_clock >>
+  gvs[UNCURRY_eq_pair] >>
+  first_x_assum $ drule_at $ Pat ‘state_rel _ _ (dec_clock _) _’ >>
+  impl_tac >- spose_not_then $ gvs o single >>
+  strip_tac >> gvs[] >>
+  gvs[AllCaseEqs(),good_res_def]
+QED
+
+Theorem OPT_MMAP_eval_correct:
+  state_rel T ctxt s t ∧
+  OPT_MMAP (eval s) argexps = SOME args ⇒
+  OPT_MMAP (eval t) (MAP (compile_exp ctxt) argexps) = SOME args
+Proof
+  rw[OPT_MMAP_MAP_o] >>
+  irule EQ_TRANS >>
+  first_assum $ irule_at $ Pos last >>
+  irule OPT_MMAP_CONG >>
+  rw[] >>
+  imp_res_tac pan_commonPropsTheory.opt_mmap_mem_func >>
+  imp_res_tac compile_exp_correct >>
+  gvs[]
+QED
+
+Theorem state_rel_lookup_code:
+  state_rel ls ctxt s t ∧
+  lookup_code s.code fname args = SOME (prog,newlocals) ⇒
+  lookup_code t.code fname args = SOME (compile ctxt prog,newlocals)
+Proof
+  rw[] >>
+  gvs[state_rel_def,lookup_code_def,AllCaseEqs()] >>
+  res_tac >> fs[]
+QED
+
+(* Simplifier doesn't trigger if flag is left symbolic *)
+Theorem state_rel_empty_locals:
+  (state_rel T ctxt s t ⇒ state_rel ls' ctxt (empty_locals s) (empty_locals t)) ∧
+  (state_rel F ctxt s t ⇒ state_rel ls' ctxt (empty_locals s) (empty_locals t))
+Proof
+  rw[] >>
+  gvs[state_rel_def,empty_locals_def]
+QED
+
+Theorem state_rel_change_locals:
+  (state_rel T ctxt s t ⇒ state_rel ls' ctxt (s with locals := x) (t with locals := x)) ∧
+  (state_rel F ctxt s t ⇒ state_rel ls' ctxt (s with locals := x) (t with locals := x))
+Proof
+  rw[] >>
+  gvs[state_rel_def,empty_locals_def]
+QED
+
+Theorem state_rel_set_var:
+  (state_rel T ctxt s t ⇒ state_rel ls' ctxt (set_var rt retv s) (set_var rt retv t))
+Proof
+  rw[] >>
+  gvs[state_rel_def,empty_locals_def,set_var_def]
+QED
+
+Theorem compile_Call:
+  ^(get_goal "compile _ (Call _ _ _)")
+Proof
+  rpt strip_tac >>
+  ‘s.clock = t.clock ∧ s.locals = t.locals’ by gvs[state_rel_def] >>
+  gvs[evaluate_def,compile_def,SF DNF_ss, good_res_def] >>
+  qpat_x_assum ‘_ = (_,_)’ mp_tac >>
+  PURE_TOP_CASE_TAC >> gvs[] >>
+  PURE_TOP_CASE_TAC >> gvs[] >>
+  imp_res_tac OPT_MMAP_eval_correct >>
+  PURE_TOP_CASE_TAC >> gvs[] >>
+  drule_all_then strip_assume_tac state_rel_lookup_code >>
+  gvs[] >>
+  IF_CASES_TAC
+  >- (rw[] >> gvs[state_rel_def,good_res_def,empty_locals_def]) >>
+  gvs[] >>
+  PURE_TOP_CASE_TAC >> gvs[] >>
+  rename1 ‘option_CASE opt’ >>
+  Cases_on ‘opt = SOME Error’ >- rw[] >>
+  first_x_assum $ drule_at $ Pos last >>
+  disch_then $ qspecl_then [‘ctxt’,‘dec_clock t with locals := r’] mp_tac >>
+  impl_keep_tac
+  >- gvs[state_rel_def,dec_clock_def] >>
+  strip_tac >>
+  rw[] >>
+  gvs[AllCaseEqs(),good_res_def,state_rel_empty_locals,PULL_EXISTS,
+      state_rel_change_locals,state_rel_set_var]
+  >- metis_tac[option_nchotomy,PAIR]
+  >- metis_tac[option_nchotomy,PAIR] >>
+  first_x_assum $ qspecl_then [‘ctxt’,‘set_var evar exn (t' with locals := t.locals)’] mp_tac >>
+  impl_keep_tac
+  >- gvs[state_rel_change_locals,state_rel_set_var] >>
+  strip_tac >>
+  simp[] >>
+  gvs[state_rel_def]
 QED
 
 Theorem resort_decls_evaluate:
